examples/CacheOblivious1D.v
@@ -18,15 +18,23 @@ End ThreePointStencil.
 Module P := Prog Z2 ThreePointStencil.
 Import P.
 
-Definition Vol (t0 t1 x0 v0 x1 v1 : Z) :=
-  (t1 - t0) * ((x1 - x0) * 2 + (v1 - v0) * (t1 - t0)).
+Definition trapezoid := (Z * Z * Z * Z * Z * Z)%type.
 
-Definition WF (t0 t1 x0 v0 x1 v1 : Z) :=
-  t0 < t1 /\
-  x0 < x1 /\
-  -1 <= v0 <= 1 /\
-  -1 <= v1 <= 1 /\
-  x0 + (t1 - t0) * v0 <= x1 + (t1 - t0) * v1.
+Definition Vol (T : trapezoid) :=
+  match T with
+    | (t0, t1, x0, v0, x1, v1) =>
+      (t1 - t0) * ((x1 - x0) * 2 + (v1 - v0) * (t1 - t0))
+  end.
+
+Definition WF (T : trapezoid) :=
+  match T with
+    | (t0, t1, x0, v0, x1, v1) =>
+      t0 < t1 /\
+      x0 < x1 /\
+      -1 <= v0 <= 1 /\
+      -1 <= v1 <= 1 /\
+      x0 + (t1 - t0) * v0 <= x1 + (t1 - t0) * v1
+  end.
 
 Ltac clear_divs :=
   repeat match goal with
@@ -44,38 +52,38 @@ Ltac clear_divs :=
 
 Lemma WF_Vol_ge0 :
   forall (t0 t1 x0 v0 x1 v1 : Z),
-    WF t0 t1 x0 v0 x1 v1 -> Vol t0 t1 x0 v0 x1 v1 >= 0.
+    WF (t0, t1, x0, v0, x1, v1) -> Vol (t0, t1, x0, v0, x1, v1) >= 0.
 Proof. unfold WF, Vol; intros; nia. Qed.
 
 Lemma WF_Vol_gt0 :
   forall (t0 t1 x0 v0 x1 v1 : Z),
-    WF t0 t1 x0 v0 x1 v1 -> Vol t0 t1 x0 v0 x1 v1 > 0.
+    WF (t0, t1, x0, v0, x1, v1) -> Vol (t0, t1, x0, v0, x1, v1) > 0.
 Proof. unfold WF, Vol; intros; nia. Qed.
 
 Lemma Spatial_cut_WF_l_general :
   forall (t0 t1 x0 v0 x1 v1 xm v : Z),
-    WF t0 t1 x0 v0 x1 v1 ->
+    WF (t0, t1, x0, v0, x1, v1) ->
     -1 <= v <= 1 ->
     x0 < xm ->
     x0 + (t1 - t0) * v0 <= xm + (t1 - t0) * v ->
-    WF t0 t1 x0 v0 xm v.
+    WF (t0, t1, x0, v0, xm, v).
 Proof. unfold WF; intuition. Qed.
 
 Lemma Spatial_cut_WF_r_general :
   forall (t0 t1 x0 v0 x1 v1 xm v : Z),
-    WF t0 t1 x0 v0 x1 v1 ->
+    WF (t0, t1, x0, v0, x1, v1) ->
     -1 <= v <= 1 ->
     xm < x1 ->
     xm + (t1 - t0) * v <= x1 + (t1 - t0) * v1 ->
-    WF t0 t1 xm v x1 v1.
+    WF (t0, t1, xm, v, x1, v1).
 Proof. unfold WF; intuition. Qed.
 
 Lemma Spatial_cut_WF_l :
   forall (t0 t1 x0 v0 x1 v1 : Z),
-    WF t0 t1 x0 v0 x1 v1 ->
+    WF (t0, t1, x0, v0, x1, v1) ->
     (t1 - t0) * 4 < (x1 - x0) * 2 + (v1 - v0) * (t1 - t0) ->
     let xm := ((x0 + x1) * 2 + (v0 + v1 + 2) * (t1 - t0)) / 4 in
-    WF t0 t1 x0 v0 xm (-1).
+    WF (t0, t1, x0, v0, xm, -1).
 Proof.
   unfold WF; intros.
   apply Spatial_cut_WF_l_general with x1 v1;
@@ -84,10 +92,10 @@ Qed.
 
 Lemma Spatial_cut_WF_r :
   forall (t0 t1 x0 v0 x1 v1 : Z),
-    WF t0 t1 x0 v0 x1 v1 ->
+    WF (t0, t1, x0, v0, x1, v1) ->
     (t1 - t0) * 4 < (x1 - x0) * 2 + (v1 - v0) * (t1 - t0) ->
     let xm := ((x0 + x1) * 2 + (v0 + v1 + 2) * (t1 - t0)) / 4 in
-    WF t0 t1 xm (-1) x1 v1.
+    WF (t0, t1, xm, -1, x1, v1).
 Proof.
   unfold WF; intros.
   apply Spatial_cut_WF_r_general with x0 v0;
@@ -96,28 +104,28 @@ Qed.
 
 Lemma Time_cut_WF_bot :
   forall (t0 t1 x0 v0 x1 v1 : Z),
-    WF t0 t1 x0 v0 x1 v1 ->
+    WF (t0, t1, x0, v0, x1, v1) ->
     t1 - t0 <> 1 ->
     (x1 - x0) * 2 + (v1 - v0) * (t1 - t0) <= (t1 - t0) * 4 ->
     let s := (t1 - t0) / 2 in
-    WF t0 (t0 + s) x0 v0 x1 v1.
+    WF (t0, t0 + s, x0, v0, x1, v1).
 Proof. unfold WF; intuition; clear_divs; intros; nia. Qed.
 
 Lemma Time_cut_WF_top :
   forall (t0 t1 x0 v0 x1 v1 : Z),
-    WF t0 t1 x0 v0 x1 v1 ->
+    WF (t0, t1, x0, v0, x1, v1) ->
     (x1 - x0) * 2 + (v1 - v0) * (t1 - t0) <= (t1 - t0) * 4 ->
     let s := (t1 - t0) / 2 in
-    WF  (t0 + s) t1 (x0 + v0 * s) v0 (x1 + v1 * s) v1.
+    WF (t0 + s, t1, x0 + v0 * s, v0, x1 + v1 * s, v1).
 Proof. unfold WF; intuition; clear_divs; intros; nia. Qed.
 
 Lemma Spatial_cut_Vol_l :
   forall (t0 t1 x0 v0 x1 v1 : Z),
-    WF t0 t1 x0 v0 x1 v1 ->
+    WF (t0, t1, x0, v0, x1, v1) ->
     t1 - t0 > 1 ->
     (t1 - t0) * 4 < (x1 - x0) * 2 + (v1 - v0) * (t1 - t0) ->
     let xm := ((x0 + x1) * 2 + (v0 + v1 + 2) * (t1 - t0)) / 4 in
-    Vol t0 t1 x0 v0 xm (-1) < Vol t0 t1 x0 v0 x1 v1.
+    Vol (t0, t1, x0, v0, xm, -1) < Vol (t0, t1, x0, v0, x1, v1).
 Proof.
   unfold WF, Vol; intuition.
   clear_divs; intros; nia.
@@ -125,11 +133,11 @@ Qed.
 
 Lemma Spatial_cut_Vol_r :
   forall (t0 t1 x0 v0 x1 v1 : Z),
-    WF t0 t1 x0 v0 x1 v1 ->
+    WF (t0, t1, x0, v0, x1, v1) ->
     t1 - t0 > 1 ->
     (t1 - t0) * 4 < (x1 - x0) * 2 + (v1 - v0) * (t1 - t0) ->
     let xm := ((x0 + x1) * 2 + (v0 + v1 + 2) * (t1 - t0)) / 4 in
-    Vol t0 t1 xm (-1) x1 v1 < Vol t0 t1 x0 v0 x1 v1.
+    Vol (t0, t1, xm, -1, x1, v1) < Vol (t0, t1, x0, v0, x1, v1).
 Proof.
   unfold WF, Vol; intuition.
   clear_divs; intros; nia.
@@ -137,24 +145,23 @@ Qed.
 
 Lemma Vol_sub_trapezoid :
   forall (t0 t1 x0 v0 x1 v1 t : Z),
-    WF t0 t1 x0 v0 x1 v1 ->
+    WF (t0, t1, x0, v0, x1, v1) ->
     t0 < t < t1 ->
-    Vol t0 t x0 v0 x1 v1 +
-    Vol t t1 (x0 + v0 * (t - t0)) v0 (x1 + v1 * (t - t0)) v1 = Vol t0 t1 x0 v0 x1 v1.
+    Vol (t0, t, x0, v0, x1, v1) +
+    Vol (t, t1, x0 + v0 * (t - t0), v0, x1 + v1 * (t - t0), v1)
+    = Vol (t0, t1, x0, v0, x1, v1).
 Proof. unfold WF, Vol; intuition; ring. Qed.
 
-Lemma silly_arith :
-  forall x y t,
-    x + t = y -> t > 0-> x < y.
+Lemma silly_arith : forall x y t, x + t = y -> t > 0-> x < y.
 Proof. intros; omega. Qed.
 
 Lemma Time_cut_Vol_bot :
   forall (t0 t1 x0 v0 x1 v1 : Z),
-    WF t0 t1 x0 v0 x1 v1 ->
+    WF (t0, t1, x0, v0, x1, v1) ->
     t1 - t0 > 1 ->
     (x1 - x0) * 2 + (v1 - v0) * (t1 - t0) <= (t1 - t0) * 4 ->
     let s := (t1 - t0) / 2 in
-    Vol t0 (t0 + s) x0 v0 x1 v1 < Vol t0 t1 x0 v0 x1 v1.
+    Vol (t0, t0 + s, x0, v0, x1, v1) < Vol (t0, t1, x0, v0, x1, v1).
 Proof.
   unfold WF; intros.
   eapply silly_arith.
@@ -166,22 +173,21 @@ Proof.
   now apply Time_cut_WF_top.
 Qed.
 
-Lemma silly_arith2 :
-  forall x y t,
-    t + x = y -> t > 0-> x < y.
+Lemma silly_arith2 : forall x y t, t + x = y -> t > 0-> x < y.
 Proof. intros; omega. Qed.
 
 Lemma Time_cut_Vol_top :
   forall (t0 t1 x0 v0 x1 v1 : Z),
-    WF t0 t1 x0 v0 x1 v1 ->
+    WF (t0, t1, x0, v0, x1, v1) ->
     t1 - t0 <> 1 ->
     (x1 - x0) * 2 + (v1 - v0) * (t1 - t0) <= (t1 - t0) * 4 ->
     let s := (t1 - t0) / 2 in
-    Vol (t0 + s) t1 (x0 + v0 * s) v0 (x1 + v1 * s) v1 < Vol t0 t1 x0 v0 x1 v1.
+    Vol (t0 + s, t1, x0 + v0 * s, v0, x1 + v1 * s, v1)
+    < Vol (t0, t1, x0, v0, x1, v1).
 Proof.
   unfold WF; intros.
   eapply silly_arith2.
-  instantiate (1 := Vol t0 (t0 + (t1 - t0) / 2) x0 v0 x1 v1).
+  instantiate (1 := Vol (t0, t0 + (t1 - t0) / 2, x0, v0, x1, v1)).
   remember ((t1 - t0) / 2) as s.
   replace (v0 * s) with (v0 * ((t0 + s) - t0)) by ring.
   replace (v1 * s) with (v1 * ((t0 + s) - t0)) by ring.
@@ -205,19 +211,16 @@ Ltac clear_reflections :=
          end.
 
 Ltac prove_WF :=
-  match goal with
-    | [ |- WF _ _ _ _ _ _ ] =>
-      clear_reflections;
-        first [now apply Spatial_cut_WF_l
-              |now apply Spatial_cut_WF_r
-              |now apply Time_cut_WF_bot
-              |now apply Time_cut_WF_top]
-  end.
+  clear_reflections;
+  first [now apply Spatial_cut_WF_l
+        |now apply Spatial_cut_WF_r
+        |now apply Time_cut_WF_bot
+        |now apply Time_cut_WF_top].
 
 Ltac prove_Vol :=
   unfold WF in * |-;
   match goal with
-    | [ |- (Z.abs_nat (Vol _ _ _ _ _ _) < Z.abs_nat (Vol _ _ _ _ _ _))%nat ] =>
+    | [ |- (Z.abs_nat _ < Z.abs_nat _)%nat ] =>
       clear_reflections;
         apply Zabs_nat_lt; split;
         [apply Z.ge_le, WF_Vol_ge0; prove_WF|];
@@ -228,32 +231,40 @@ Ltac prove_Vol :=
         (assumption || omega)
   end.
 
-Local Obligation Tactic := program_simpl; (prove_WF || prove_Vol).
+Arguments Zminus m n : simpl never.
+Local Obligation Tactic := program_simpl; try (prove_WF || prove_Vol).
 
-Program Fixpoint Walk1 (t0 t1 x0 v0 x1 v1 : Z)
-        (H : WF t0 t1 x0 v0 x1 v1)
-        {measure (Z.abs_nat (Vol t0 t1 x0 v0 x1 v1))} :=
-  let h := t1 - t0 in
-  (if dec (h =? 1) then
-     For "x" From x0 To (x1 - 1) Do
-       Fire (t0 : aexpr, "x" : aexpr)
-   else
-     if dec (h * 4 <? (x1 - x0) * 2 + (v1 - v0) * h) then
-       let xm := ((x0 + x1) * 2 + (v0 + v1 + 2) * h) / 4 in
-       Walk1 t0 t1 x0 v0 xm (-1) _;;
-       Walk1 t0 t1 xm (-1) x1 v1 _
-     else
-       let s := h / 2 in
-       Walk1 t0 (t0 + s) x0 v0 x1 v1 _;;
-       Walk1 (t0 + s) t1 (x0 + v0 * s) v0 (x1 + v1 * s) v1 _)%prog.
+Program Fixpoint Walk1 (Tp : trapezoid | WF Tp) {measure (Z.abs_nat (Vol Tp))} :=
+  match Tp with
+    | (t0, t1, x0, v0, x1, v1) =>
+      let h := t1 - t0 in
+      if dec (h =? 1) then
+        For "x" From x0 To (x1 - 1) Do
+          Fire (t0 : aexpr, "x" : aexpr)
+      else
+        if dec (h * 4 <? (x1 - x0) * 2 + (v1 - v0) * h) then
+          let xm := ((x0 + x1) * 2 + (v0 + v1 + 2) * h) / 4 in
+          Walk1 (@exist _ _ (t0, t1, x0, v0, xm, -1) _);;
+          Walk1 (@exist _ _ (t0, t1, xm, -1, x1, v1) _)
+        else
+          let s := h / 2 in
+          Walk1 (@exist _ _ (t0, t0 + s, x0, v0, x1, v1) _);;
+          Walk1 (@exist _ _ (t0 + s, t1, x0 + v0 * s, v0, x1 + v1 * s, v1) _)
+  end%prog.
 
-(*Section Walk1_correct.
-  Variables t0 t1 x0 v0 x1 v1.
-  Hypothesis Ht : t0 < t1.
-  Hypothesis Hx : x0 < x1.
-  Hypothesis Hv0 : -1 <= v0 <= 1.
-  Hypothesis Hv1 : -1 <= v1 <= 1.
+Example WF_ex :
+  WF (0,5,0,0,5,0).
+Proof. unfold WF; intuition omega. Qed.
 
-  Theorem Walk1_shape :
-      shape (Walk1 t0 t1 x0 v0 x1 v1) ≡
-            ⋃⎨〚x0 + v0 * (t - t0), x0 + v1 * (t - t0)〛, t ∈〚t0, t1〛⎬.*)
+Eval compute in psimpl (Walk1 (@exist _ _ (0, 5, 0, 0, 5, 0) WF_ex)).
+
+(*Theorem Walk1_shape :
+  forall t0 t1 x0 v0 x1 v1 v
+         (H : WF (t0, t1, x0, v0, x1, v1)),
+    shape v (Walk1 (@exist _ _ (t0, t1, x0, v0, x1, v1) H)) ≡
+          (⋃⎨⎨(x0 + v0 * (t - t0), x0 + v1 * (t - t0))⎬, t ∈〚t0, t1〛⎬).
+Proof.
+  intros.
+  compute.
+  unfold Walk1, Fix_sub, Walk1_obligation_9.
+  induction (Z.)*)
