sources/Automation.v
@@ -1,13 +1,146 @@
-Require Import List ZArith.
-Require Import Psatz.
+Require Import List ZArith Psatz.
 Import ListNotations.
 Local Open Scope Z_scope.
 
 Require Import Sets.
 
+Ltac inv H := inversion H; subst; clear H.
 
-(** * Bruteforce existentials instantiation *)
+Tactic Notation "decide" constr(x) "=" constr(y) :=
+  destruct (Z.eq_dec x y); subst; simpl in *.
 
+(** * First automation layer: Simplifying goals. *)
+
+Ltac simplify_hyps :=
+  repeat
+    match goal with
+      | [ H : @is_in _ _ (@empty _) |- _ ] => inv H
+      | [ H : @is_in _ _ (@singleton _ _) |- _ ] => inv H
+      | [ H : @is_in _ _ (@segment _ _) |- _ ] => inv H
+      | [ H : @is_in _ _ (@bin_union _ _ _) |- _ ] => inv H
+      | [ H : @is_in _ _ (@times _ _ _ _) |- _ ] => inv H
+      | [ H : @is_in _ _ (@param_union _ _ _ _) |- _ ] => inv H
+
+      | [ H : @empty _ _ |- _] => inversion H
+      | [ H : @singleton _ _ _ |- _ ] => red in H
+      | [ H : @segment _ _ _ |- _ ] => red in H
+      | [ H : @bin_union _ _ _ _ |- _ ] => red in H
+      | [ H : @times _ _ _ _ _ |- _ ] => destruct H
+      | [ H : @param_union _ _ _ _ _ |- _ ] => destruct H as [? [? ?]]
+
+      | [ x : @prod _ _ |- _ ] => destruct x
+
+      | [ H : _ /\ _ |- _ ] => destruct H
+      | [ H : _ \/ _ |- _ ] => destruct H
+end.
+
+Ltac simplify_goal' :=
+  match goal with
+    | [ |- @subset _ _ _ ] => intro
+
+    | [ |- @is_in _ _ (@singleton _ _) ] =>
+      constructor; red
+    | [ |- @is_in _ _ (@segment _ _) ] =>
+      constructor; split
+    | [ |- @is_in _ (@pair _ _ _ _) (@times _ _ _ _) ] =>
+      constructor; split
+    | [ |- @is_in _ _ (@param_union _ _ _ _) ] =>
+      constructor; red
+
+    | [ H : @same _ ?A _ |- @is_in _ _ ?A ] => now apply H
+    | [ H : @same _ _ ?A |- @is_in _ _ ?A ] => now apply H
+
+    | [ |- forall _, _ ] => intro
+    | [ |- _ /\ _ ] => split
+    | [ |- _ <-> _ ] => split
+    | [ |- ~ _ ] => intro
+
+    | [ x : @prod _ _ |- _ ] => destruct x
+    | [ |- @pair _ _ _ _ = @pair _ _ _ _ ] => f_equal
+  end.
+
+Ltac simplify_goal :=
+  repeat progress simplify_goal'.
+
+Ltac double_incl := match goal with [ |- @same _ _ _ ] => intro end.
+
+Ltac forward :=
+  repeat
+    first [assumption | reflexivity |
+           progress simplify_goal | progress simplify_hyps | double_incl].
+
+(** [step] does set theoretic reasoning.  [lhs] and [rhs] allow one to prove
+ * that an element belongs to a binary union, by proving that it belongs to one
+ * of the two given sets. *)
+
+Ltac lhs :=
+  match goal with
+    [ |- @is_in _ _ (@bin_union _ _ _) ] => constructor; left
+  end.
+
+Ltac rhs :=
+  match goal with
+      [ |- @is_in _ _ (@bin_union _ _ _) ] => constructor; right
+  end.
+
+Ltac forward' :=
+  repeat first [lhs; now forward' | rhs; now forward' |
+                progress forward].
+
+(** * Bruteforce pass-or-fail automation. *)
+
+Ltac iter_exists l tac :=
+  match l with
+    | ?x :: ?xs =>
+      (exists x; tac) || iter_exists xs tac
+  end.
+
+(* [bruteforce' l] tries to solve the current goal.  If needed, it
+ * instanciates existential variables using the variables provided in [l]. *)
+
+Ltac bruteforce' l :=
+  simplify_hyps;
+  match goal with
+    | [ |- @subset _ _ _ ] => intro; bruteforce' l
+
+    | [ |- @is_in _ _ (@singleton _ _) ] =>
+      constructor; red; bruteforce' l
+    | [ |- @is_in _ _ (@segment _ _) ] =>
+      constructor; split; bruteforce' l
+    | [ |- @is_in _ (@pair _ _ _ _) (@times _ _ _ _) ] =>
+      constructor; split; bruteforce' l
+    | [ |- @is_in _ _ (@bin_union _ _ _) ] =>
+      (lhs; bruteforce' l) || (rhs; bruteforce' l)
+    | [ |- @is_in _ _ (@param_union _ _ _ _) ] =>
+      constructor; red; bruteforce' l
+
+    | [ |- forall _, _ ] =>
+      intro; bruteforce' l
+    | [ |- exists _, _ ] =>
+      iter_exists l ltac:(bruteforce' l)
+    | [ |- ~ _ ] =>
+      intro; bruteforce' l
+    | [ |- _ /\ _ ] =>
+      split; bruteforce' l
+    | [ |- _ \/ _ ] =>
+      (left; bruteforce' l) || (right; bruteforce' l)
+    | [ H : _ \/ _ |- _ ] =>
+      destruct H; bruteforce' l
+
+    | [ |- False ] =>
+      simpl in *; nia
+    | [ |- _ <= _ ] =>
+      simpl in *; nia
+    | [ |- _ = _ ] =>
+      simpl in *; nia
+    | [ |- _ = _ ] =>
+      progress f_equal; bruteforce' l
+  end.
+
+Ltac bruteforce :=
+  bruteforce' ([] : list Z).
+
+(** * Generating all expressions from a list of constants. *)
 
 (** The following few functions are used to generate a list of ALL expressions
  * of depth at most [n], using constants from a list [l] and operators from a
@@ -47,75 +180,3 @@ Fixpoint gen_expr' l ops (n : nat) acc :=
   end.
 Definition gen_expr l ops n :=
   rev' (gen_expr' l ops n l).
-
-
-(** ******************************************************************** *)
-
-Tactic Notation "decide" constr(x) "=" constr(y) :=
-  destruct (Z.eq_dec x y); subst; simpl in *.
-
-Ltac inv H := inversion H; subst; clear H.
-
-Ltac simplify_set_hyps :=
-  repeat
-    match goal with
-      | [ H : @is_in _ _ (@empty _) |- _ ] => inv H
-      | [ H : @is_in _ _ (@singleton _ _) |- _ ] => inv H
-      | [ H : @is_in _ _ (@segment _ _) |- _ ] => inv H
-      | [ H : @is_in _ _ (@bin_union _ _ _) |- _ ] => inv H
-      | [ H : @is_in _ _ (@times _ _ _ _) |- _ ] => inv H
-      | [ H : @is_in _ _ (@param_union _ _ _ _) |- _ ] => inv H
-
-      | [ H : @empty _ _ |- _] => inversion H
-      | [ H : @singleton _ _ _ |- _ ] => red in H
-      | [ H : @segment _ _ _ |- _ ] => red in H
-      | [ H : @bin_union _ _ _ _ |- _ ] => red in H
-      | [ H : @times _ _ _ _ _ |- _ ] => destruct H
-      | [ H : @param_union _ _ _ _ _ |- _ ] => destruct H as [? [? ?]]
-    end.
-
-Ltac iter_exists l tac :=
-  match l with
-    | ?x :: ?xs =>
-      (exists x; tac) || iter_exists xs tac
-  end.
-
-Ltac bruteforce' l :=
-  simplify_set_hyps;
-  match goal with
-    | [ |- @is_in _ _ (@singleton _ _) ] =>
-      constructor; red; bruteforce' l
-    | [ |- @is_in _ _ (@segment _ _) ] =>
-      constructor; split; bruteforce' l
-    | [ |- @is_in _ (@pair _ _ _ _) (@times _ _ _ _) ] =>
-      constructor; split; bruteforce' l
-    | [ |- @is_in _ _ (@bin_union _ _ _) ] =>
-      (lhs; bruteforce' l) || (rhs; bruteforce' l)
-    | [ |- @is_in _ _ (@param_union _ _ _ _) ] =>
-      constructor; red; bruteforce' l
-
-    | [ |- forall _, _ ] =>
-      intro; bruteforce' l
-    | [ |- exists _, _ ] =>
-      iter_exists l ltac:(bruteforce' l)
-    | [ |- ~ _ ] =>
-      intro; bruteforce' l
-    | [ |- _ /\ _ ] =>
-      split; bruteforce' l
-    | [ |- _ \/ _ ] =>
-      (left; bruteforce' l) || (right; bruteforce' l)
-    | [ H : _ \/ _ |- _ ] =>
-      destruct H; bruteforce' l
-
-    | [ |- False ] =>
-      simpl in *; nia
-    | [ |- _ <= _ ] =>
-      simpl in *; nia
-    | [ |- _ = _ ] =>
-      simpl in *; nia
-    | [ |- _ = _ ] =>
-      progress f_equal; bruteforce' l
-  end.
-
-Ltac bruteforce :=
-  bruteforce' ([] : list Z).
