sources/Problems.v
@@ -5,6 +5,7 @@ Module Type DOMAIN.
   Parameter cell : Type.
   Parameter cexpr : Type.
   Parameter ceval : vars -> cexpr -> cell.
+  Parameter csimpl : cexpr -> cexpr.
 
 End DOMAIN.
 
