sources/SetsFacts.v
@@ -1,0 +1,118 @@
+Require Import ZArith Setoid Morphisms.
+Local Open Scope Z_scope.
+Require Import Sets Automation.
+Local Open Scope set_scope.
+
+(** The main rewriting system.  We prove compatibility of set theoretic operations
+ * with [same] and prove a few identities, which are bundled in the [sets]
+ * rewriting hints database. *)
+
+Instance same_E : forall {U}, Equivalence (@same U).
+Proof. firstorder. Qed.
+
+Instance same_is_in_Proper :
+  forall U, Proper (eq ==> same ==> iff) (@is_in U).
+Proof.
+  unfold Proper, respectful.
+  split; intros; subst; firstorder.
+Qed.
+
+Instance subset_is_in_Proper :
+  forall U, Proper (same ==> same ==> iff) (@subset U).
+Proof. unfold Proper, respectful; firstorder. Qed.
+
+Instance same_bin_union_Proper :
+  forall U, Proper (same ==> same ==> same) (@bin_union U).
+Proof. unfold Proper, respectful. forward'. Qed.
+
+Instance same_times_Proper :
+  forall U V, Proper (same ==> same ==> same) (@times U V).
+Proof. unfold Proper, respectful; forward. Qed.
+
+Instance same_param_union_Proper :
+  forall U a b, Proper (pointwise_relation _ same ==> same) (@param_union U a b).
+Proof.
+  unfold Proper, respectful, pointwise_relation.
+  forward; exists x1; forward; now apply H.
+Qed.
+
+Lemma bin_union_empty_l :
+  forall U (A : set U), ∅ ∪ A ≡ A.
+Proof. forward'. Qed.
+Hint Rewrite bin_union_empty_l : set_setoid.
+
+Lemma bin_union_empty_r :
+  forall U (A : set U), A ∪ ∅ ≡ A.
+Proof. forward'. Qed.
+Hint Rewrite bin_union_empty_r : set_setoid.
+
+Lemma bin_union_idem :
+  forall U (A : set U), A ∪ A ≡ A.
+Proof. forward'. Qed.
+Hint Rewrite bin_union_idem : set_setoid.
+
+Lemma times_empty_l :
+  forall U V (A : set V), (∅ : set U) × A ≡ ∅.
+Proof. forward. Qed.
+Hint Rewrite times_empty_l : set_setoid.
+
+Lemma times_empty_r :
+  forall U V (A : set U), A × (∅ : set V) ≡ ∅.
+Proof. forward. Qed.
+Hint Rewrite times_empty_r : set_setoid.
+
+Lemma param_union_singleton :
+  forall a b, ⋃⎨⎨k⎬, k ∈〚a, b〛⎬ ≡ 〚a, b〛.
+Proof.
+  forward; [now subst | now subst | ].
+  exists x; forward.
+Qed.
+Hint Rewrite param_union_singleton : set_setoid.
+
+Lemma param_union_singleton_l :
+  forall U (B : set U) a b, ⋃ ⎨ ⎨k⎬ × B, k ∈〚a, b〛⎬ ≡ 〚a, b〛× B.
+Proof.
+  forward.
+  unfold fst, snd in *; now subst.
+  unfold fst, snd in *; now subst.
+  exists z; forward.
+Qed.
+Hint Rewrite param_union_singleton_l : set_setoid.
+
+Lemma param_union_singleton_r :
+  forall U (A : set U) a b, ⋃ ⎨ A × ⎨k⎬, k ∈〚a, b〛⎬ ≡ A ×〚a, b〛.
+Proof.
+  forward.
+  unfold fst, snd in *; now subst.
+  unfold fst, snd in *; now subst.
+  exists z; forward.
+Qed.
+Hint Rewrite param_union_singleton_r : set_setoid.
+
+Tactic Notation "simplify" "sets" "with" reference(l) :=
+  unfold l; simpl;
+  repeat
+    first
+    [ setoid_rewrite bin_union_empty_l
+    | setoid_rewrite bin_union_empty_r
+    | setoid_rewrite bin_union_idem
+    | setoid_rewrite times_empty_l
+    | setoid_rewrite times_empty_r
+    | setoid_rewrite param_union_singleton
+    | setoid_rewrite param_union_singleton_l
+    | setoid_rewrite param_union_singleton_r].
+
+Lemma param_union_bin :
+  forall U a b (A : Z -> set U),
+    a <= b -> ⋃ ⎨ A k, k ∈〚a, b〛⎬ ≡ ⋃ ⎨ A k, k ∈〚a, b-1〛⎬ ∪ A b.
+Proof.
+  forward.
+  + decide x0=b; subst; [rhs | lhs]; forward.
+  exists x0; forward; omega.
+  + (exists x0; forward; omega).
+  + (exists b; forward; omega).
+Qed.
+
+Lemma bin_union_assoc :
+  forall U (A B C : set U), (A ∪ B) ∪ C ≡ A ∪ (B ∪ C).
+Proof. forward'. Qed.
